lean4/Koika.lean
@@ -12,5 +12,6 @@ import Koika.Semantics.Interp
 import Koika.Compile.Lowered
 import Koika.Compile.Circuit
 import Koika.Compile.Lower
+import Koika.Compile.Optimize
 import Koika.Backend.Verilog
 import Koika.Basic
